lib_list/ArrayListGen.fsti
@@ -1,0 +1,308 @@
+module ArrayListGen
+
+open Steel.Memory
+open Steel.Effect.Atomic
+open Steel.Effect
+open Steel.ArrayRef
+
+module A = Steel.Array
+module L = FStar.List.Tot
+module US = FStar.SizeT
+module FS = FStar.FiniteSet.Base
+open FStar.FiniteSet.Ambient
+
+(** A library for doubly linked lists, that are located in memory in a contiguous region (an array) *)
+
+/// The type of cells for the doubly linked list. Compared to a standard doubly linked list,
+/// the `prev` and `next` fields are not pointers, but offsets in the array containing the list.
+/// To keep unsigned (positive) integers, we will represent NULL as 0, and not store anything
+/// in the first element slot of the array
+val cell (t:Type0) : Type0
+
+inline_for_extraction noextract
+val get_data (#a:Type0) (c:cell a) : a
+
+/// As a convention, we represent NULL as 0
+noextract inline_for_extraction
+let null : nat = 0
+noextract inline_for_extraction
+let null_ptr : US.t = 0sz
+
+/// The toplevel specification of being a list
+/// When [hd] is the head pointer of the list, the set of visited nodes
+/// is initially empty, and the prev "pointer" should be "NULL"
+val is_dlist (#a:Type0) (pred: a -> prop)  (hd:nat) (s:Seq.seq (cell a)) : prop
+
+/// Offset [x] belongs to the list starting at [hd]
+val mem (#a:Type0) (x:nat) (hd:nat) (s:Seq.seq (cell a)) : prop
+
+/// An alternative specification for belonging to the list,
+/// `ptrs_in` returns the set of elements in the list starting
+/// at [hd]
+val ptrs_in (#a:Type) (hd:nat) (s:Seq.seq (cell a)) : GTot (FS.set nat)
+
+/// Set of all pointers contained in the three doubly linked lists
+let ptrs_all (#a:Type) (hd1 hd2 hd3:nat) (s:Seq.seq (cell a)) =
+  FS.union (ptrs_in hd1 s) (FS.union (ptrs_in hd2 s) (ptrs_in hd3 s))
+
+/// Membership of element [x] in any of the dlist pointed to by [hd1], [hd2], or [hd3]
+let mem_all (#a:Type0) (x:nat) (hd1 hd2 hd3:nat) (s:Seq.seq (cell a)) =
+  FS.mem x (ptrs_all hd1 hd2 hd3 s)
+
+/// Equivalence lemma between `mem` and membership in `ptrs_in`
+val lemma_mem_ptrs_in (#a:Type)
+  (hd: nat)
+  (s: Seq.seq (cell a))
+  (x: nat)
+  : Lemma (mem x hd s <==> FS.mem x (ptrs_in hd s))
+
+/// Disjointness between two lists, specified directly on the sets of pointers
+/// to alleviate the need for recursive reasoning
+val disjoint (#a:Type)
+  (s: Seq.seq (cell a))
+  (hd1 hd2: nat)
+  : prop
+
+/// Mutual exclusiveness for three dlists
+let disjoint3 (#a:Type) (s:Seq.seq (cell a)) (hd1 hd2 hd3: nat) =
+  disjoint s hd1 hd2 /\ disjoint s hd1 hd3 /\ disjoint s hd2 hd3
+
+/// The array is partitioned exactly between the three lists
+let partition (#a:Type) (s:Seq.seq (cell a)) (hd1 hd2 hd3: nat) =
+  forall (i:nat{i < Seq.length s}). i == null \/ (FS.mem i (ptrs_all hd1 hd2 hd3 s))
+
+(** Some helpers to use cells *)
+
+val read_data (#a:Type) (c:cell a) : a
+
+val write_data (#a:Type0) (c:cell a) (v:a) : cell a
+
+(** Steel functions and vprops *)
+
+/// The refinement predicate for varraylist, stating that the sequence contains
+/// three mutually exclusive doubly linked lists
+let varraylist_refine (#a:Type)
+  (pred1 pred2 pred3: a -> prop)
+  (hd1 hd2 hd3:nat)
+  (s:Seq.seq (cell a)) : prop
+  = is_dlist pred1 hd1 s /\ is_dlist pred2 hd2 s /\ is_dlist pred3 hd3 s /\ disjoint3 s hd1 hd2 hd3
+
+/// The main vprop of this module.
+/// We have access to an array, such that the array contains three mutually
+/// exclusive doubly linked list, starting at offsets [hd1] [hd2] and [hd3]
+/// respectively
+[@@__steel_reduce__]
+let varraylist (#a:Type) (pred1 pred2 pred3: a -> prop) (r:A.array (cell a)) (hd1 hd2 hd3:nat) : vprop
+  = A.varray r `vrefine` (varraylist_refine pred1 pred2 pred3 hd1 hd2 hd3)
+
+/// Create an arraylist with
+val intro_arraylist_nil (#a:Type) (#opened:inames)
+  (pred1 pred2 pred3: a -> prop)
+  (r:A.array (cell a))
+  (hd1 hd2 hd3:US.t) :
+  SteelGhost unit opened
+    (A.varray r)
+    (fun _ -> varraylist pred1 pred2 pred3 r (US.v hd1) (US.v hd2) (US.v hd3))
+    (requires fun _ ->
+      A.length r == 0 /\
+      hd1 == null_ptr /\
+      hd2 == null_ptr /\
+      hd3 == null_ptr)
+    (ensures fun _ _ h1 ->
+      h1 (varraylist pred1 pred2 pred3 r (US.v hd1) (US.v hd2) (US.v hd3)) `Seq.equal` Seq.empty
+    )
+
+/// Reads at index [idx] in the array.
+inline_for_extraction noextract
+val read_in_place (#a:Type)
+  (#pred1 #pred2 #pred3: a -> prop)
+  (r:A.array (cell a))
+  (hd1 hd2 hd3:Ghost.erased nat)
+  (idx:US.t{US.v idx < A.length r})
+  : Steel a
+          (varraylist pred1 pred2 pred3 r hd1 hd2 hd3)
+          (fun _ -> varraylist pred1 pred2 pred3 r hd1 hd2 hd3)
+          (requires fun _ -> True)
+          (ensures fun h0 _ h1 ->
+            h0 (varraylist pred1 pred2 pred3 r hd1 hd2 hd3) ==
+            h1 (varraylist pred1 pred2 pred3 r hd1 hd2 hd3))
+
+/// Updates the `data` field of the cell at index [idx] in the array [r] with [v]
+/// We define three different functions, depending on which list the element
+/// belongs to. In all three cases, we require [v] to satisfy the predicate
+/// corresponding to a given list
+inline_for_extraction noextract
+val write_in_place1 (#a:Type)
+  (#pred1 #pred2 #pred3: a -> prop)
+  (r:A.array (cell a))
+  (hd1 hd2 hd3:Ghost.erased nat)
+  (idx:US.t{US.v idx < A.length r})
+  (v:a)
+   : Steel unit
+          (varraylist pred1 pred2 pred3 r hd1 hd2 hd3)
+          (fun _ -> varraylist pred1 pred2 pred3 r hd1 hd2 hd3)
+          (requires fun h -> pred1 v /\ mem (US.v idx) hd1 (h (varraylist pred1 pred2 pred3 r hd1 hd2 hd3)))
+          (ensures fun h0 _ h1 -> True) // TODO
+
+inline_for_extraction noextract
+val write_in_place2 (#a:Type)
+  (#pred1 #pred2 #pred3: a -> prop)
+  (r:A.array (cell a))
+  (hd1 hd2 hd3:Ghost.erased nat)
+  (idx:US.t{US.v idx < A.length r})
+  (v:a)
+   : Steel unit
+          (varraylist pred1 pred2 pred3 r hd1 hd2 hd3)
+          (fun _ -> varraylist pred1 pred2 pred3 r hd1 hd2 hd3)
+          (requires fun h -> pred2 v /\ mem (US.v idx) hd2 (h (varraylist pred1 pred2 pred3 r hd1 hd2 hd3)))
+          (ensures fun h0 _ h1 -> True) // TODO
+
+inline_for_extraction noextract
+val write_in_place3 (#a:Type)
+  (#pred1 #pred2 #pred3: a -> prop)
+  (r:A.array (cell a))
+  (hd1 hd2 hd3:Ghost.erased nat)
+  (idx:US.t{US.v idx < A.length r})
+  (v:a)
+   : Steel unit
+          (varraylist pred1 pred2 pred3 r hd1 hd2 hd3)
+          (fun _ -> varraylist pred1 pred2 pred3 r hd1 hd2 hd3)
+          (requires fun h -> pred3 v /\ mem (US.v idx) hd3 (h (varraylist pred1 pred2 pred3 r hd1 hd2 hd3)))
+          (ensures fun h0 _ h1 -> True) // TODO
+
+/// Removes the element at offset [idx] from the dlist pointed to by [hd1]
+inline_for_extraction noextract
+val remove1 (#a:Type)
+  (#pred1 #pred2 #pred3: a -> prop)
+  (r:A.array (cell a))
+  (hd1:US.t)
+  (hd2 hd3:Ghost.erased nat)
+  (idx:US.t{US.v idx < A.length r})
+   : Steel US.t
+          (varraylist pred1 pred2 pred3 r (US.v hd1) hd2 hd3)
+          (fun hd' -> varraylist pred1 pred2 pred3 r (US.v hd') hd2 hd3)
+          (requires fun h -> mem (US.v idx) (US.v hd1) (h (varraylist pred1 pred2 pred3 r (US.v hd1) hd2 hd3)))
+          (ensures fun h0 hd' h1 ->
+            ptrs_in (US.v hd') (h1 (varraylist pred1 pred2 pred3 r (US.v hd') hd2 hd3)) ==
+            FS.remove (US.v idx) (ptrs_in (US.v hd1) (h0 (varraylist pred1 pred2 pred3 r (US.v hd1) hd2 hd3))) /\
+            ptrs_in hd2 (h1 (varraylist pred1 pred2 pred3 r (US.v hd') hd2 hd3)) ==
+            ptrs_in hd2 (h0 (varraylist pred1 pred2 pred3 r (US.v hd1) hd2 hd3)) /\
+            ptrs_in hd3 (h1 (varraylist pred1 pred2 pred3 r (US.v hd') hd2 hd3)) ==
+            ptrs_in hd3 (h0 (varraylist pred1 pred2 pred3 r (US.v hd1) hd2 hd3))
+          )
+
+/// Removes the element at offset [idx] from the dlist pointed to by [hd2]
+inline_for_extraction noextract
+val remove2 (#a:Type)
+  (#pred1 #pred2 #pred3: a -> prop)
+  (r:A.array (cell a))
+  (hd1:Ghost.erased nat)
+  (hd2:US.t)
+  (hd3:Ghost.erased nat)
+  (idx:US.t{US.v idx < A.length r})
+   : Steel US.t
+          (varraylist pred1 pred2 pred3 r hd1 (US.v hd2) hd3)
+          (fun hd' -> varraylist pred1 pred2 pred3 r hd1 (US.v hd') hd3)
+          (requires fun h -> mem (US.v idx) (US.v hd2) (h (varraylist pred1 pred2 pred3 r hd1 (US.v hd2) hd3)))
+          (ensures fun h0 hd' h1 ->
+            ptrs_in (US.v hd') (h1 (varraylist pred1 pred2 pred3 r hd1 (US.v hd') hd3)) ==
+            FS.remove (US.v idx) (ptrs_in (US.v hd2) (h0 (varraylist pred1 pred2 pred3 r hd1 (US.v hd2) hd3))) /\
+            ptrs_in hd1 (h1 (varraylist pred1 pred2 pred3 r hd1 (US.v hd') hd3)) ==
+            ptrs_in hd1 (h0 (varraylist pred1 pred2 pred3 r hd1 (US.v hd2) hd3)) /\
+            ptrs_in hd3 (h1 (varraylist pred1 pred2 pred3 r hd1 (US.v hd') hd3)) ==
+            ptrs_in hd3 (h0 (varraylist pred1 pred2 pred3 r hd1 (US.v hd2) hd3))
+          )
+
+/// Removes the element at offset [idx] from the dlist pointed to by [hd3]
+inline_for_extraction noextract
+val remove3 (#a:Type)
+  (#pred1 #pred2 #pred3: a -> prop)
+  (r:A.array (cell a))
+  (hd1 hd2:Ghost.erased nat)
+  (hd3:US.t)
+  (idx:US.t{US.v idx < A.length r})
+   : Steel US.t
+          (varraylist pred1 pred2 pred3 r hd1 hd2 (US.v hd3))
+          (fun hd' -> varraylist pred1 pred2 pred3 r hd1 hd2 (US.v hd'))
+          (requires fun h -> mem (US.v idx) (US.v hd3) (h (varraylist pred1 pred2 pred3 r hd1 hd2 (US.v hd3))))
+          (ensures fun h0 hd' h1 ->
+            ptrs_in (US.v hd') (h1 (varraylist pred1 pred2 pred3 r hd1 hd2 (US.v hd'))) ==
+            FS.remove (US.v idx) (ptrs_in (US.v hd3) (h0 (varraylist pred1 pred2 pred3 r hd1 hd2 (US.v hd3)))) /\
+            ptrs_in hd1 (h1 (varraylist pred1 pred2 pred3 r hd1 hd2 (US.v hd'))) ==
+            ptrs_in hd1 (h0 (varraylist pred1 pred2 pred3 r hd1 hd2 (US.v hd3))) /\
+            ptrs_in hd2 (h1 (varraylist pred1 pred2 pred3 r hd1 hd2 (US.v hd'))) ==
+            ptrs_in hd2 (h0 (varraylist pred1 pred2 pred3 r hd1 hd2 (US.v hd3)))
+          )
+
+/// Requires that the element at offset [idx] does not belong to any dlist.
+/// If so, insert it at the head of list [hd1]
+inline_for_extraction noextract
+val insert1 (#a:Type)
+  (#pred1 #pred2 #pred3: a -> prop)
+  (r:A.array (cell a))
+  (hd:US.t{hd == null_ptr \/ US.v hd < A.length r})
+  (hd2 hd3:Ghost.erased nat)
+  (idx:US.t{idx <> null_ptr /\ US.v idx < A.length r})
+  (v: a)
+   : Steel unit
+          (varraylist pred1 pred2 pred3 r (US.v hd) hd2 hd3)
+          (fun _ -> varraylist pred1 pred2 pred3 r (US.v idx) hd2 hd3)
+          (requires fun h -> pred1 v /\
+            (~ (mem_all (US.v idx) (US.v hd) hd2 hd3 (h (varraylist pred1 pred2 pred3 r (US.v hd) hd2 hd3)))))
+          (ensures fun h0 hd' h1 ->
+            ptrs_in (US.v idx) (h1 (varraylist pred1 pred2 pred3 r (US.v idx) hd2 hd3)) ==
+            FS.insert (US.v idx) (ptrs_in (US.v hd) (h0 (varraylist pred1 pred2 pred3 r (US.v hd) hd2 hd3))) /\
+            ptrs_in hd2 (h1 (varraylist pred1 pred2 pred3 r (US.v idx) hd2 hd3)) ==
+            ptrs_in hd2 (h0 (varraylist pred1 pred2 pred3 r (US.v hd) hd2 hd3)) /\
+            ptrs_in hd3 (h1 (varraylist pred1 pred2 pred3 r (US.v idx) hd2 hd3)) ==
+            ptrs_in hd3 (h0 (varraylist pred1 pred2 pred3 r (US.v hd) hd2 hd3))
+          )
+
+
+/// Requires that the element at offset [idx] does not belong to any dlist.
+/// If so, insert it at the head of list [hd2]
+inline_for_extraction noextract
+val insert2 (#a:Type)
+  (#pred1 #pred2 #pred3: a -> prop)
+  (r:A.array (cell a))
+  (hd:US.t{hd == null_ptr \/ US.v hd < A.length r})
+  (hd1 hd3:Ghost.erased nat)
+  (idx:US.t{idx <> null_ptr /\ US.v idx < A.length r})
+  (v: a)
+   : Steel unit
+          (varraylist pred1 pred2 pred3 r hd1 (US.v hd) hd3)
+          (fun _ -> varraylist pred1 pred2 pred3 r hd1 (US.v idx) hd3)
+          (requires fun h -> pred2 v /\
+            (~ (mem_all (US.v idx) hd1 (US.v hd) hd3 (h (varraylist pred1 pred2 pred3 r hd1 (US.v hd) hd3)))))
+          (ensures fun h0 hd' h1 ->
+            ptrs_in (US.v idx) (h1 (varraylist pred1 pred2 pred3 r hd1 (US.v idx) hd3)) ==
+            FS.insert (US.v idx) (ptrs_in (US.v hd) (h0 (varraylist pred1 pred2 pred3 r hd1 (US.v hd) hd3))) /\
+            ptrs_in hd1 (h1 (varraylist pred1 pred2 pred3 r hd1 (US.v idx) hd3)) ==
+            ptrs_in hd1 (h0 (varraylist pred1 pred2 pred3 r hd1 (US.v hd) hd3)) /\
+            ptrs_in hd3 (h1 (varraylist pred1 pred2 pred3 r hd1 (US.v idx) hd3)) ==
+            ptrs_in hd3 (h0 (varraylist pred1 pred2 pred3 r hd1 (US.v hd) hd3))
+          )
+
+/// Requires that the element at offset [idx] does not belong to any dlist.
+/// If so, insert it at the head of list [hd3]
+inline_for_extraction noextract
+val insert3 (#a:Type)
+  (#pred1 #pred2 #pred3: a -> prop)
+  (r:A.array (cell a))
+  (hd:US.t{hd == null_ptr \/ US.v hd < A.length r})
+  (hd1 hd2:Ghost.erased nat)
+  (idx:US.t{idx <> null_ptr /\ US.v idx < A.length r})
+  (v: a)
+   : Steel unit
+          (varraylist pred1 pred2 pred3 r hd1 hd2 (US.v hd))
+          (fun _ -> varraylist pred1 pred2 pred3 r hd1 hd2 (US.v idx))
+          (requires fun h -> pred3 v /\
+            (~ (mem_all (US.v idx) hd1 hd2 (US.v hd) (h (varraylist pred1 pred2 pred3 r hd1 hd2 (US.v hd))))))
+          (ensures fun h0 hd' h1 ->
+            ptrs_in (US.v idx) (h1 (varraylist pred1 pred2 pred3 r hd1 hd2 (US.v idx))) ==
+            FS.insert (US.v idx) (ptrs_in (US.v hd) (h0 (varraylist pred1 pred2 pred3 r hd1 hd2 (US.v hd)))) /\
+            ptrs_in hd1 (h1 (varraylist pred1 pred2 pred3 r hd1 hd2 (US.v idx))) ==
+            ptrs_in hd1 (h0 (varraylist pred1 pred2 pred3 r hd1 hd2 (US.v hd))) /\
+            ptrs_in hd2 (h1 (varraylist pred1 pred2 pred3 r hd1 hd2 (US.v idx))) ==
+            ptrs_in hd2 (h0 (varraylist pred1 pred2 pred3 r hd1 hd2 (US.v hd)))
+          )
